update example: work around
- Demonstate a wordaround for bug https://dafny.codeplex.com/workitem/144

dafny-bug-existential-predicate.dfy
@@ -1,19 +1,47 @@
 ﻿/**
- * Demonstrate a bug of Dafny described in https://dafny.codeplex.com/workitem/144
+ * Demonstrate a bug of Dafny and its workaround.
+ * See https://dafny.codeplex.com/workitem/144 for details.
  */
 
 class ExistentiallyQuantifiedPredicateBug
 {
 	var arr : array<int>;
-	predicate p(i:int)
+
+	predicate p(i: int)
+
 	method foo()
 		requires arr != null && arr.Length > 0
 		modifies arr
 	{
 		assume exists i :: p(i);
+		ghost var i :| p(i);
 		arr[0] := 1;
-		assert exists i :: p(i); // FAILS
+		assert p(i);
+		assert exists i :: p(i); // FAILS without assert p(i)
 	}
+
+	predicate q(i: int, j: int)
+
+	predicate q'(i: int)
+		requires arr != null && arr.Length > 0
+		reads this`arr
+	{
+		exists j | 0 <= j < arr.Length :: q(i, j)
+	}
+
+	method goo()
+		requires arr != null && arr.Length > 0
+		modifies arr
+	{
+		assume forall i | 0 <= i < arr.Length :: q'(i);
+		var i := 0;
+		while i < arr.Length {
+			assert q'(i);
+			arr[i] := i;
+			i := i + 1;
+		}
+	}
+
 }
 
 predicate p(i:int)
@@ -21,15 +49,13 @@ predicate p(i:int)
 method m3()
 
 method m1()
-	// a workaround
-	requires exists i :: p(i)
-	ensures exists i :: p(i) 
 {}
 
 method m2()
 {
   assume exists i :: p(i);
-  assert exists i :: p(i);
+  ghost var i :| p(i);
   m1();
-  assert exists i :: p(i); // FAILS without workaround
+  assert p(i);
+  assert exists i :: p(i); // FAILS without assert p(i)
 }
